Tidy

examples/steel/StructRef.fst
@@ -3,71 +3,39 @@ module StructRef
 open FStar.PCM
 module M = Steel.Memory
 
+(** Very well-behaved lenses *)
 noeq type lens (a: Type u#a) (b: Type u#b) = {
   get: a -> b;
   put: b -> a -> a;
-  get_put: s: a -> v: b -> Lemma (get (put v s) == v); // [SMTPat (get (put v s))];
-  put_get: s: a -> Lemma (put (get s) s == s); // [SMTPat (put (get s) s)];
-  put_put: s: a -> v: b -> w: b -> Lemma (put v (put w s) == put v s); // [SMTPat (put v (put w s))];
+  get_put: s: a -> v: b -> Lemma (get (put v s) == v);
+  put_get: s: a -> Lemma (put (get s) s == s);
+  put_put: s: a -> v: b -> w: b -> Lemma (put v (put w s) == put v s);
 }
-
 let get_put' (l: lens 'a 'b) (s: 'a) (v: 'b)
   : Lemma (l.get (l.put v s) == v) [SMTPat (l.get (l.put v s))]
   = l.get_put s v
-
 let put_get' (l: lens 'a 'b) (s: 'a)
   : Lemma (l.put (l.get s) s == s) [SMTPat (l.put (l.get s))]
   = l.put_get s
-
 let put_put' (l: lens 'a 'b) (s: 'a) (v w: 'b)
   : Lemma (l.put v (l.put w s) == l.put v s) [SMTPat (l.put v (l.put w s))]
   = l.put_put s v w
 
-let upd (l: lens 'a 'b) (f: 'b -> 'b) (s: 'a): 'a = l.put (f (l.get s)) s
+(** Updating the target of a lens *)
+let lens_upd (l: lens 'a 'b) (f: 'b -> 'b) (s: 'a): 'a = l.put (f (l.get s)) s
 
-(* The non-computational part of frame_preserving_upd *)
-let frame_pres (p: pcm 'a) (f: 'a -> 'a) (x y: Ghost.erased 'a) =
-  forall (v:'a{p.refine v /\ compatible p x v}).{:pattern compatible p x v}
-  p.refine (f v) /\
-  compatible p y (f v) /\
-  (forall (frame:'a{composable p x frame}).{:pattern composable p x frame}
-     composable p y frame /\
-     (op p x frame == v ==> op p y frame == f v))
-
-(* Every function satisfying frame_pres is a frame_preserving_upd *)
-let frame_pres_mk_upd (p: pcm 'a) (x y: Ghost.erased 'a)
-  (f:('a -> 'a){frame_pres p f x y})
-  : frame_preserving_upd p x y
-  = fun v -> f v
-
-(* A pcm_lens is a lens for a 'b inside an 'a such that upd lifts
-   frame-preserving updates on 'b to frame-preserving updates on 'a *)
-noeq type pcm_lens (#a: Type u#a) (#b: Type u#b) (p: pcm a) (q: pcm b) = {
-  raw: lens a b;
-  upd_resp_pcm:
-    s: a -> v: b -> f:(b -> b) ->
-    Lemma
-      (requires frame_pres q f (raw.get s) v)
-      (ensures frame_pres p (upd raw f) s (raw.put v s));
-}
-
-let upd_resp_pcm' (p: pcm 'a) (q: pcm 'b) (l: pcm_lens p q) (s: 'a) (v: 'b) (f: 'b -> 'b)
-  : Lemma
-      (requires frame_pres q f (l.raw.get s) v)
-      (ensures frame_pres p (upd l.raw f) s (l.raw.put v s))
-      [SMTPat (frame_pres q f (l.raw.get s) v)]
-  = l.upd_resp_pcm s v f
-
-(* A ref is a pcm_lens combined with a Steel.Memory.ref for the base type 'a *)
-noeq type ref (#a: Type u#a) (#b: Type u#b) (p: pcm a) (q: pcm b) = {
-  l: pcm_lens p q;
-  r: M.ref a p;
+let const (x: 'a) (b: 'b): 'a = x
+let lens_id #a : lens a a = {
+  get = id;
+  put = const;
+  get_put = (fun _ _ -> ());
+  put_get = (fun _ -> ());
+  put_put = (fun _ _ _ -> ());
 }
 
 let get_comp (l: lens 'a 'b) (m: lens 'b 'c) (s: 'a): 'c = m.get (l.get s)
 let put_comp (l: lens 'a 'b) (m: lens 'b 'c) (v: 'c) (s: 'a): 'a =
-  upd l (m.put v) s
-
+  lens_upd l (m.put v) s
 let lens_comp (l: lens 'a 'b) (m: lens 'b 'c): lens 'a 'c = {
   get = get_comp l m;
   put = put_comp l m;
@@ -76,8 +44,52 @@ let lens_comp (l: lens 'a 'b) (m: lens 'b 'c): lens 'a 'c = {
   put_put = (fun _ _ _ -> ());
 }
 
-let pcm_lens_comp (#p: pcm 'a) (#q: pcm 'b) (#r: pcm 'c)
-  (l: pcm_lens p q) (m: pcm_lens q r) : pcm_lens p r = {
-  raw = lens_comp l.raw m.raw;
-  upd_resp_pcm = (fun _ _ _ -> ());
+(** The non-computational part of frame_preserving_upd
+    TODO: move this and lemmas about this to FStar.PCM.fst *)
+let frame_pres (p: pcm 'a) (f: 'a -> 'a) (x y: Ghost.erased 'a) =
+  forall (v:'a{p.refine v /\ compatible p x v}).{:pattern compatible p x v}
+  p.refine (f v) /\
+  compatible p y (f v) /\
+  (forall (frame:'a{composable p x frame}).{:pattern composable p x frame}
+     composable p y frame /\
+     (op p x frame == v ==> op p y frame == f v))
+
+(** Every function satisfying frame_pres is a frame_preserving_upd *)
+let frame_pres_mk_upd (p: pcm 'a) (x y: Ghost.erased 'a)
+  (f:('a -> 'a){frame_pres p f x y})
+  : frame_preserving_upd p x y
+  = fun v -> f v
+
+(** Given PCMs (p: pcm a) and (q: pcm b), a (pcm_lens p q) is a (lens a b)
+    with the extra law that lens_upd lifts frame-preserving updates on
+    b w.r.t. q to frame-preserving updates on a w.r.t. p. *)
+noeq type pcm_lens (#a: Type u#a) (#b: Type u#b) (p: pcm a) (q: pcm b) = {
+  raw: lens a b;
+  upd_resp_pcm: s: a -> v: b -> f:(b -> b) ->
+    Lemma
+      (requires frame_pres q f (raw.get s) v)
+      (ensures frame_pres p (lens_upd raw f) s (raw.put v s));
 }
+let upd_resp_pcm' (p: pcm 'a) (q: pcm 'b) (l: pcm_lens p q) (s: 'a) (v: 'b) (f: 'b -> 'b)
+  : Lemma
+      (requires frame_pres q f (l.raw.get s) v)
+      (ensures frame_pres p (lens_upd l.raw f) s (l.raw.put v s))
+      [SMTPat (frame_pres q f (l.raw.get s) v)]
+  = l.upd_resp_pcm s v f
+
+let pcm_lens_id (#p: pcm 'a): pcm_lens p p
+  = {raw = lens_id; upd_resp_pcm = (fun _ _ _ -> ())}
+let pcm_lens_comp (#p: pcm 'a) (#q: pcm 'b) (#r: pcm 'c)
+  (l: pcm_lens p q) (m: pcm_lens q r): pcm_lens p r
+  = {raw = lens_comp l.raw m.raw; upd_resp_pcm = (fun _ _ _ -> ())}
+
+let get (#p: pcm 'a) (#q: pcm 'b) (l: pcm_lens p q) (s: 'a): 'b = l.raw.get s
+let put (#p: pcm 'a) (#q: pcm 'b) (l: pcm_lens p q) (v: 'b) (s: 'a): 'a = l.raw.put v s
+let upd (#p: pcm 'a) (#q: pcm 'b) (l: pcm_lens p q) (f: 'b -> 'b) (s: 'a): 'a = lens_upd l.raw f s
+
+(* A ref is a pcm_lens combined with a Steel.Memory.ref for the base type 'a *)
+noeq type ref (#a: Type u#a) (#b: Type u#b) (p: pcm a) (q: pcm b) = {
+  l: pcm_lens p q;
+  r: M.ref a p;
+}
+
